\documentclass[class=scrartcl, crop=false]{standalone}

\usepackage[sexy]{evan}
\usepackage{cole}

% \documentclass{article}
% 
% \usepackage{amsmath}
% \usepackage{amssymb}
% \usepackage{enumerate}
% \usepackage{parskip}
% \usepackage{siunitx}
% \usepackage{tikz}
% \usepackage{upgreek}
% \usepackage[margin=0.5in]{geometry}
% \usepackage{graphicx}
% \usepackage{esint}
% \usepackage{nicematrix}
% \NiceMatrixOptions{transparent}

\begin{document}

\title{Notes 2019-09-11}
\author{Cole Killian}


Pitfall of proof in the wrong direction.

\subsection{ex. $\forall x \geq y \geq 0: \sqrt{x - y} \geq \sqrt{x} - \sqrt{y}$}

$\Leftrightarrow x - y \geq (\sqrt{x} - \sqrt{y})^2 = x-2 \sqrt{x} \sqrt{y} + y$

\end{document}
