\documentclass[class=scrartcl, crop=false]{standalone}

\usepackage[sexy]{/home/gautierk/.config/evan}


\begin{document}

\section{Tutorial 10-30}


\subsection{e}

\begin{example}
  
  \begin{enumerate}
    \ii[]
    \ii
    \begin{gather*}
      \lim(1 - \frac{1}{n})^{-n} = e
    \end{gather*}
    \ii
    \begin{gather*}
      (1 + \frac{1}{2n})^n = ((1 + \frac{1}{2n})^{2n})^\frac{1}{2} = (e)^\frac{1}{2}
    \end{gather*}
    Because $(1 + \frac{1}{2n})$ is a subsequence of $(1 + \frac{1}{n})$ which converges to e.
    \ii
    $(1 + \frac{n}{2})^{\frac{n}{2}}$ is \ul{not} a subsequence of $(1 + \frac{1}{n})^n$. It's the other way around.

  \end{enumerate}
\end{example}

Let $a > 0$. Pick $x_1 > 0$. Let $x_{n + 1} = \frac{1}{2}(x_n + \frac{a}{x_n}) > 0$ 
\\\\
Prove that $x_n \to \sqrt{a}$.

\end{document}
