
\documentclass{article}

\usepackage{amsmath}
\usepackage{amssymb}
\usepackage{enumerate}
\usepackage{parskip}
\usepackage{siunitx}
\usepackage{tikz}
\usepackage{upgreek}
\usepackage[margin=0.5in]{geometry}
\usepackage{graphicx}
\usepackage{esint}
\usepackage{nicematrix}
\NiceMatrixOptions{transparent}

\begin{document}

\title{Notes 2019-09-11}
\author{Cole Killian}


\section{Mathematical Induction}

Suppose have sequence of statements: $S_1, S_2, \dots \{S_n: n \in \mathbb{N}\}$

Principle of mathematical induction:

Suppose  $S_1$ is true (base case)

Suppose $S_n \Rightarrow S_{n+1}$ for each n (the induction)

Then $S_n$ is true for each $n \in \mathbb{N}$ 

ex. $\int_n = 1 + 2 + 3 + \dots + n = \frac{n(n+1)}{2}$

(base case) $S_1:  1 = \frac{1(1 + 1)}{2}$

(induction) $S_n \Rightarrow S_{n+1}$

$S_n: 1 + 2 + \dots + n = \frac{n(n+1)}{2}$

$\ \ \ \ \ +n + 1$

$S_n: 1 + 2 + \dots + n + (n + 1) = \frac{n(n+1)}{2} + (n + 1)$

\end{document}
