\documentclass[class=scrartcl, crop=false]{standalone}

\usepackage[sexy]{evan}
\usepackage{cole}


\date{2020-03-11}


\begin{document}

\section{Lecture 03-11}

\subsection{Inner product spaces}

$V$ over $F = \RR, \CC$.

\begin{enumerate}
  \ii
  Positivity:
  \begin{gather*}
    \lang v, v \rang \in \RR \geq 0 \\
    \lang v, v \rang = 0 \Leftrightarrow v = 0
  \end{gather*} 
  \ii
  Rather than imposing bilinearity, we were lead to impose hermition linearity.
  \ii
  Basic symmetry assumption requiring the $\lang v, w \rang = \ol{\lang w, v \rang}$.
  \ii
  We defined norm of $v$ as 
\begin{gather*}
  ||v|| = \sqrt{\lang, v, v \rang}
\end{gather*} 
\end{enumerate} 


\begin{theorem}[Cauchy-Schwartz Inequality]
  For all $v, w \in V$,
  \begin{gather*}
    |\lang v, w \rang | \leq ||v|| \cdot ||w||
    \\
    \ \text{With equal if } \ \spn(v, w) \ \text{is one dimensional} \ 
  \end{gather*} 
  \begin{proof}
    We can assume without loss of generality that $v \neq 0$.
    \\\\
    Positivity implies that for all $\lambda \in F$,
    \begin{gather*} % review these
      \lang \lambda v + w, \lambda v + w \rang \in \RR \geq 0 \\
      = |\lambda|^2\lang v, v \rang + \lambda \lang v, w \rang + \ol{\lambda}\lang w, v \rang + \lang w, w, \rang \geq 0 \\
      |\lambda|^2 \lang v, v, \rang + 2 Re(\lambda \lang v, w \rang ) + \lang w, w, \rang \geq 0, \quad \forall \lambda \in F
    \end{gather*} 
    \begin{enumerate}
      \ii
      If $F = \RR$.
      \begin{gather*}
        f(\lambda) = \lambda^2 \lang v, v \rang + 2 \lang v, w \rang \lambda + \lang w, w \rang \geq 0, \quad \forall \lambda \in \RR \\
        \ \text{This is a quadratic so either it has a root or it doesn't} \ 
        \\
        \Rightarrow (2 \lang v, w \rang )^2 - 4 \lang v, v, \rang \lang w, w, \rang \leq 0 \\
        \ \text{with equal if there is a root} \ 
        \\
        \Rightarrow \lang v, w \rang ^2 \leq ||v||^2||w||^2 \\
        \Rightarrow |\lang v, w \rang | \leq ||v||||w|| \\
        \ \text{with equal if} \ \exists \lambda_0 \ \text{such that} \ f(\lambda) = 0 \\
        i.e. \ \lang \lambda_0 v + w, \lambda_0v + w \rang = 0 \Rightarrow 
        \lambda_0v + w = 0 \Rightarrow \spn(v, w) = \spn(v) \ \checkmark
      \end{gather*} 
      \ii
      If $F = \CC$. Assume that $\lambda \lang v, w \rang \in \RR$.
      \begin{gather*}
        |\lambda|^2 \lang v, v \rang \pm 2 |\lambda|| \lang v, w \rang | + \lang w, w, \rang \geq 0
        \\
        \ \text{Doesn't matter on the sign because b term squared in discriminant} \ 
        \\
        4| \lang v, w \rang |^2 - 4 \lang v, v \rang \lang w, w \rang \leq 0 \\
        \Rightarrow |\lang v, w \rang |^2 \leq ||v||^2||w||^2
      \end{gather*} 
      The rest follows like the real case.
    \end{enumerate} 
  \end{proof} 
\end{theorem} 

\subsection{Properties of $||v||$}
\begin{enumerate}
  \ii
  \begin{gather*}
    ||v|| \in \RR \geq 0
  \end{gather*} 
  \ii
  \begin{gather*}
    ||\lambda v|| = |\lambda| \cdot ||v||
  \end{gather*} 
  \ii
  \begin{gather*}
    ||v + w || \leq ||v|| + ||w|| \ \text{with equality if} \ (v, w) \ \text{are colinear.} \ 
  \end{gather*} 
\end{enumerate} 
\begin{proof}
  \begin{enumerate}
    \ii[]
    \ii
    By definition
    \ii
    \begin{gather*}
      ||\lambda v || = \sqrt{\lang \lambda v, \lambda v \rang} = \sqrt{\lambda \ol{\lambda}}\sqrt{\lang v, v \rang} = |\lambda| \cdot ||v||
    \end{gather*} 
    \ii % Review 2Re term
    \begin{gather*}
      ||v + w||^2 = \lang v + w, v + w \rang = ||v||^2 + 2Re \lang v, w \rang + ||w||^2 \\
      \leq ||v||^2 + 2|\lang v, w \rang | + ||w||^2, \quad \ \text{because} \ Re(\lambda) \leq |\lambda| \\
      \leq ||v||^2 + 2||v||||w|| + ||w||^2 = (||v|| + ||w||)^2 \\
      \Rightarrow ||v + w|| \leq ||v|| + ||w||
    \end{gather*} 
  \end{enumerate} 
\end{proof} 

\begin{definition}[Orthogonality]
  Two vectors are \ul{orthogonal} if $\lang v, w \rang = 0$.
\end{definition} 

\begin{definition}[Orthonormal Basis]
  An orthonormal basis of $V$ is a basis $\Sigma$ of $V$ such that for all $v, w \in \Sigma$, 
  \begin{gather*}
    \lang v, w \rang = 
    \begin{cases}
      0, & \ \text{if} \ v \neq w \\
      1, & \ \text{if} \ v = w
    \end{cases} 
  \end{gather*} 
\end{definition}  
\begin{example}
  \begin{enumerate}
    \ii[]
    \ii
    $V = \RR^n$ or $\CC^n$ with dot product. 
    \begin{gather*}
      e_1 = (1, 0, \dots, 0), \ e_2 = (0, 1, \dots, 0), \ e_n = (0, 0, \dots, 1)
    \end{gather*} 
    is an orthonormal basis.
    \ii
    $V = P_n([0, 1])$, the space of polynomials of degree $\leq n$ with 
    \begin{gather*}
      \lang f, g \rang = \int_0^1 f(t) \ol{g(t)} dt
    \end{gather*} 
    Then
    \begin{gather*}
      \Sigma = (1, x, x^2, \dots, x^n)
    \end{gather*} 
    is \ul{not} an orthonormal basis because inner product is not zero pairwise between these elements
  \end{enumerate} 
\end{example} 

\begin{theorem}
  If $V$ is a finite-dimensional inner product space over $\RR$ or $\CC$, then it has an orthonormal basis.
  \begin{proof}
    We will prove something more precise. Let $(v_1, \dots, v_n)$ be a basis for $V$, then there is $(e_1, \dots, e_n)$ orthonormal with 
    \begin{gather*}
      \spn(e_1, \dots, e_j) = \spn(v_1, \dots, v_j), \quad j = 1, \dots, n
    \end{gather*} 
    We will prove the existence of $(e_1, \dots, e_n)$ by induction on $j$.
    \begin{enumerate}
      \ii
      Base case $j = 1$, let $ e_1 = v_1 / ||v_1||$.
      \ii
      Inductive step $j \to j + 1$. Assume that we have an orthonormal collection $ e_1, \dots, e_j$ with $\spn(e_1, \dots, e_j)$, with $\spn(e_1, \dots, e_j) = \spn(v_1, \dots, v_j)$. We then must define $e_{j + 1}$.
      \begin{gather*}
        \widetilde{e_{j + 1}} = \lambda_1e_1 + \lambda_2e_2 + \cdots + \lambda_ie_i + \lambda_{j + 1}v_{j + 1}
      \end{gather*} 
      Want $\widetilde{e_{j + 1}} \perp e_i, \quad i = 1, \dots, j$.
      \begin{gather*}
        0 = \lang \widetilde{e_{j + 1}}, e_i \rang = \lambda_i + \lambda_{j + 1}\lang v_{j + 1}, e_i \rang \\
        \lambda_i = -\lambda_{j + 1} \lang v_{j + 1}, e_i \rang
      \end{gather*} 
      Set $\lambda_{j + 1} = 1$, then $\lambda_i = -\lang v_{j + 1}, e_i \rang$.
      \begin{gather*}
        \widetilde{e_{j + 1}} = v_{j+ 1} - \lang v_{j + 1}, e_1 \rang e_1 + \cdots + \lang v_{j + 1}, e_j \rang e_j
      \end{gather*} 
      is orthogonal to $e_1, \dots, e_j$ and hence $ v_1, \dots, v_j$.
      \begin{gather*}
        e_{j + 1} = \widetilde{e_{j + 1}} \frac{1}{||\widetilde{e_{j + 1}}}
      \end{gather*} 
    \end{enumerate} 
  \end{proof} 
\end{theorem} 

\end{document}
